\noindent\textbf{Solution 1}\\\\

\textbf{Claim:} $\triangle BPR\sim\triangle BAC$\\
Dem: Veamos que $\angle PBR = 45^{o} + \angle ABR = \angle RBC + \angle ABR = \angle ABC$.
Por otra parte como  $\triangle RBC\sim\triangle PBA$ tenemos que $\frac{PB}{BR}=\frac{AB}{BC}$ y queda probado el claim.

Ahora, 

\begin{equation*}
\begin{split}
\angle RPA +\angle PAQ & = (\angle APB-\angle RPB) + (\angle BAP +\angle CAB + \angle QAC) \\
& = (90^{o}-\angle CAB) + (45^{o}+\angle CAB+ 45^{o}) \\
& = 180^{o}
\end{split}   
\end{equation*}

esto implica que $PR\parallel AQ$, an√°logamoente $QR\parallel AP$.